Speed up memory allocator, yielding a large performance increase.
The next_key function we were using to find the largest address in
memory had to iterate through every element in the map. Now we search
through the BST for the largest key efficiently.

Previously running data/yarpgenv2/link/test1.ll took ~68s. With this
update it takes ~15s.

src/coq/Utils/IntMaps.v
@@ -166,19 +166,251 @@ Section Map_Operations.
     | None => false
     end.
 
+  Fixpoint IM_raw_greatest_key {A} (m : IM.Raw.tree A) : option Z
+    := match m with
+       | IM.Raw.Leaf => None
+       | IM.Raw.Node l k _ (@IM.Raw.Leaf _) _ =>
+           ret k
+       | IM.Raw.Node l k _ r _ =>
+           IM_raw_greatest_key r
+       end.
+
+  Definition IM_greatest_key {A} (m : IM.t A) : option Z
+    := IM_raw_greatest_key (IM.this m).
+
   Definition next_key {A} (m : IntMap A) : Z
+    := match IM_greatest_key m with
+       | Some k => 1 + k
+       | None => 0
+       end.
+
+  Definition next_key_old {A} (m : IntMap A) : Z
     := let keys := map fst (IM.elements m) in
        1 + maximumBy Z.leb (-1)%Z keys.
 
-  Lemma next_key_gt_0 :
+  Lemma next_key_old_gt_0 :
     forall {A} (m : IntMap A),
-      next_key m >= 0.
+      next_key_old m >= 0.
   Proof using.
     intros A m.
-    unfold next_key.
+    unfold next_key_old.
     pose proof maximumBy_Z_def (-1) (map fst (IM.elements (elt:=A) m)).
     apply Zle_is_le_bool in H.
     lia.
+  Qed.
+
+  Lemma IM_greatest_key_none' :
+    forall {A} (m : IM.t A), IM.Empty m -> IM_greatest_key m = None.
+  Proof.
+    intros A m H.
+    induction m; cbn in *.
+    induction this; cbn in *; auto.
+    - exfalso; eapply H.
+      cbn.
+      constructor; reflexivity.
+  Qed.
+
+  Lemma IM_greatest_key_none'' :
+    forall {A} (m : IM.t A), IM_greatest_key m = None -> IM.Empty m.
+  Proof.
+    intros A m H.
+    induction m; cbn in *.
+    induction this; cbn in *; auto.
+    - intros k e CONTRA.
+      inv CONTRA.
+    - exfalso.
+      destruct (IM_raw_greatest_key this2) eqn:THIS2.
+      + break_match_hyp_inv.
+      + break_match_hyp_inv.
+        inv is_bst.
+        specialize (IHthis2 H5 eq_refl).
+        eapply IHthis2.
+        constructor; reflexivity.
+  Qed.
+
+  Lemma IM_greatest_key_none :
+    forall {A} (m : IM.t A), IM_greatest_key m = None <-> IM.Empty m.
+  Proof.
+    intros A m.
+    split; intros H.
+    + apply IM_greatest_key_none''; auto.
+    + apply IM_greatest_key_none'; auto.
+  Qed.
+
+  Lemma IM_greatest_key_In :
+    forall {A} (m : IM.t A) gk,
+      IM_greatest_key m = Some gk -> IM.In gk m.
+  Proof.
+    intros A m.
+    intros gk H.
+    apply F.in_find_iff.
+    revert gk H.
+    destruct m; cbn in *.
+    induction this; intros gk GK.
+    - cbn in *. inv GK.
+    - rename k into current_key.
+      cbn.
+      (* gk is the greatest key. It should be larger than current_key *)
+      cbn in GK.
+      pose proof is_bst as is_bst2.
+      inv is_bst.
+      destruct (IM_raw_greatest_key this2) eqn:THIS2;
+        destruct this2; inv GK.
+      + (* At a leaf eq *)
+        break_match; cbn in *;
+          solve
+            [ red in l; lia
+            | discriminate
+            ].
+      + (* Not at a leaf... *)
+        pose proof H5.
+        eapply IHthis2 in H5; eauto.
+        eapply IM.Raw.Proofs.find_in_iff in H5; eauto.
+
+        red in H7.
+        apply H7 in H5.
+
+        break_match; cbn in *;
+          try solve
+            [ red in l; lia
+            | discriminate
+            ].
+
+        apply IHthis2; auto.
+      + break_match; cbn in *;
+          solve
+            [ red in l; lia
+            | discriminate
+            ].
+  Qed.
+
+  Lemma IM_greatest_key_In' :
+    forall {A} (m : IM.t A) k,
+      IM.In k m ->
+      exists gk, IM_greatest_key m = Some gk.
+  Proof.
+    intros A m k IN.
+    destruct (IM_greatest_key m) eqn:GK.
+    exists z; auto.
+
+    apply F.in_find_iff in IN.
+    destruct (IM.find (elt:=A) k m) eqn:FIND; try contradiction.
+    apply F.find_mapsto_iff in FIND.
+    apply IM_greatest_key_none in FIND; try contradiction; auto.
+  Qed.
+
+  Lemma IM_greatest_key_lt :
+    forall {A} (m : IM.t A) gk,
+      IM_greatest_key m = Some gk -> IM.Raw.lt_tree (1 + gk) (IM.this m).
+  Proof.
+    intros A m.
+    destruct m; cbn in *.
+    induction this; intros gk GK.
+    - cbn in *. inv GK.
+    - rename k into current_key.
+      cbn.
+      (* gk is the greatest key. It should be larger than current_key *)
+      cbn in GK.
+      pose proof is_bst as is_bst2.
+      inv is_bst.
+      destruct (IM_raw_greatest_key this2) eqn:THIS2;
+        destruct this2; inv GK.
+      + (* At a leaf eq *)
+        break_match; cbn in *;
+          solve
+            [ red in l; lia
+            | discriminate
+            ].
+      + (* Not at a leaf... *)
+        pose proof H5.
+        eapply IHthis2 in H5; eauto.
+        red.
+        intros y H0.
+        inv H0.
+        * (* Root *)
+          red in H5.
+          specialize (H5 k).
+          forward H5.
+          constructor; auto.
+          specialize (H7 k).
+          forward H7.
+          constructor; auto.
+          cbn in H7.
+          lia.
+        * (* Left *)
+          red in H6.
+          specialize (H6 y H2).
+          red in H5.
+          specialize (H5 k).
+          forward H5.
+          constructor; auto.
+          specialize (H7 k).
+          forward H7.
+          constructor; auto.
+          cbn in H7.
+          lia.
+        * (* Right *)
+          red in H5.
+          specialize (H5 y H2).
+          auto.
+      + red.
+        intros y H.
+        assert (gk < 1 + gk) by lia.
+        inv H; auto.
+        * apply H6 in H2.
+          cbn in *; lia.
+        * inv H2.
+  Qed.
+
+
+  Lemma IM_raw_greatest_key_lr :
+    forall {elt} m k (e : elt) l t r kl kr,
+      IM.this m = (IM.Raw.Node l k e r t) ->
+      IM_raw_greatest_key l = Some kl ->
+      IM_raw_greatest_key r = Some kr ->
+      kl < kr.
+  Proof.
+    intros elt m k e l t r kl kr NODE GL GR.
+    destruct m.
+    cbn in *.
+    inv is_bst.
+    inv H.
+    inv H3.
+
+    unfold IM.Raw.gt_tree in *.
+    unfold IM.Raw.lt_tree in *.
+
+    assert (IM_greatest_key (@IM.Bst elt l H) = Some kl) as GL' by (cbn; auto).
+    assert (IM_greatest_key (@IM.Bst elt r H0) = Some kr) as GR' by (cbn; auto).
+
+    apply IM_greatest_key_In in GL', GR'.
+    unfold IM.In in *.
+    apply IM.Raw.Proofs.In_alt in GL', GR'.
+    apply H2 in GR'.
+    apply H1 in GL'.
+
+    lia.
+  Qed.
+
+  Lemma next_key_correct :
+    forall {A} (m : IM.t A) (a : Z),
+      IM.In a m ->
+      (a < next_key m)%Z.
+  Proof.
+    intros A m a IN.
+    pose proof IN as GK.
+    unfold next_key.
+    eapply IM_greatest_key_In' in GK.
+    destruct GK as (gk & GK).
+    rewrite GK.
+    apply IM_greatest_key_lt in GK.
+    red in GK.
+    specialize (GK a).
+    destruct m; cbn in IN.
+    unfold IM.In in IN.
+    apply IM.Raw.Proofs.In_alt in IN.
+    apply GK in IN.
+    auto.
   Qed.
 
   Lemma MapsTo_inj : forall {a} k v v' (m : IntMap a),
